interpolations: eliminated axioms inject_perm_nonempty and extends_perm_nonempty.
linking_extension: added simple type anntotation, to
 ensure file processes in Coq8.3.

sepcomp/mem_interpolation_EI.v
@@ -1,10 +1,8 @@
 Load loadpath.
-(*CompCert imports*) 
 
 Require Import Events. (*is needed for some definitions (loc_unmapped etc, and
   also at the very end of this file, in order to convert between the 
-  tweaked and the standard definitions of mem_unchanged_on etc, and for
-  being able to remove/add inject_permorder/extends_permorder etc*)
+  tweaked and the standard definitions of mem_unchanged_on etc*)
 Require Import Memory.
 Require Import Coqlib.
 Require Import Integers.
@@ -12,16 +10,21 @@ Require Import Values.
 Require Import Maps.
 
 Require Import sepcomp.mem_lemmas.
-Require Import sepcomp.mem_interpolation_defs.
+Require Import sepcomp.i_defs.
 
-Definition AccessMap_EI_Property  (m1 m1' m2 : mem)
+Definition AccessMap_EI_Property (j:meminj) (m1 m1' m2 : mem)
            (AM:ZMap.t (Z -> perm_kind -> option permission)):Prop :=
   forall b2, 
     (Mem.valid_block m2 b2 -> forall k ofs2,
-         (Mem.perm m1 b2 ofs2 Max Nonempty -> 
+       match j b2 with 
+         None => ZMap.get b2 AM ofs2 k  = 
+                        ZMap.get b2 m2.(Mem.mem_access) ofs2 k
+       | Some (b3,d3) =>
+          (Mem.perm m1 b2 ofs2 Max Nonempty -> 
            ZMap.get b2 AM ofs2 k = ZMap.get b2 m1'.(Mem.mem_access) ofs2 k) 
        /\ (~Mem.perm m1 b2 ofs2 Max Nonempty -> 
-           ZMap.get b2 AM ofs2 k  = ZMap.get b2 m2.(Mem.mem_access) ofs2 k))
+           ZMap.get b2 AM ofs2 k  = ZMap.get b2 m2.(Mem.mem_access) ofs2 k)
+     end)
   /\ (~ Mem.valid_block m2 b2 -> forall k ofs2,
          (Mem.perm m1' b2 ofs2 Max Nonempty ->
            ZMap.get b2 AM ofs2 k = ZMap.get b2 m1'.(Mem.mem_access) ofs2 k)
@@ -31,30 +34,30 @@ Definition Content_EI_Property (j:meminj) (m1 m1' m2:Mem.mem)
                                (CM:ZMap.t (ZMap.t memval)):=
   forall b2, 
       (Mem.valid_block m2 b2 -> forall ofs2,
-         (Mem.perm m1 b2 ofs2 Max Nonempty -> 
              match j b2 with
-                 Some (b3,delta3) => ZMap.get ofs2 (ZMap.get b2 CM) =
-                          ZMap.get ofs2 (ZMap.get b2 m1'.(Mem.mem_contents))
-              | None => ZMap.get ofs2 (ZMap.get b2 CM) = 
-                        ZMap.get ofs2 (ZMap.get b2 m2.(Mem.mem_contents))
-               end)
-    /\ (~Mem.perm m1 b2 ofs2 Max Nonempty -> 
-            ZMap.get ofs2 (ZMap.get b2 CM) = 
-            ZMap.get ofs2 (ZMap.get b2 m2.(Mem.mem_contents))))
+               None =>  ZMap.get ofs2 (ZMap.get b2 CM) =
+                           ZMap.get ofs2 (ZMap.get b2 m2.(Mem.mem_contents))
+             | Some (b3,delta3) => 
+                     (Mem.perm m1 b2 ofs2 Max Nonempty ->
+                            ZMap.get ofs2 (ZMap.get b2 CM) =
+                           ZMap.get ofs2 (ZMap.get b2 m1'.(Mem.mem_contents)))
+                 /\ (~Mem.perm m1 b2 ofs2 Max Nonempty -> 
+                          ZMap.get ofs2 (ZMap.get b2 CM) = 
+                         ZMap.get ofs2 (ZMap.get b2 m2.(Mem.mem_contents)))
+            end)
   /\ (~ Mem.valid_block m2 b2 -> forall ofs2,
-           (Mem.perm m1' b2 ofs2 Max Nonempty ->
+           (Mem.perm m1' b2 ofs2 Cur Readable ->
                 ZMap.get ofs2 (ZMap.get b2 CM) =
                 ZMap.get ofs2 (ZMap.get b2 m1'.(Mem.mem_contents)))
-        /\ (~Mem.perm m1' b2 ofs2 Max Nonempty -> 
+        /\ (~Mem.perm m1' b2 ofs2 Cur Readable -> 
                 ZMap.get ofs2 (ZMap.get b2 CM) =Undef)).
 
 Lemma EI_ok: forall (m1 m2 m1':mem)
-               (Ext12: Mem.extends m1 m2) (EP12: extends_perm_nonempty m1 m2)
+               (Ext12: Mem.extends m1 m2)
                (Fwd1: mem_forward m1 m1') m3 j
-               (Inj23: Mem.inject j m2 m3) (IP23: inject_perm_nonempty j m2 m3)
+               (Inj23: Mem.inject j m2 m3)
                m3' (Fwd3: mem_forward m3 m3') j'
                (Inj13': Mem.inject j' m1' m3')
-               (IP13': inject_perm_nonempty j' m1' m3')
                (UnchOn3: my_mem_unchanged_on (loc_out_of_reach j m1) m3 m3') 
                (InjInc: inject_incr j j') (injSep: inject_separated j j' m1 m3)
                (UnchOn1: my_mem_unchanged_on (loc_unmapped j) m1 m1')
@@ -62,53 +65,25 @@ Lemma EI_ok: forall (m1 m2 m1':mem)
                (WD2: mem_wd m2) (WD3': mem_wd m3') m2'
                (NB: m2'.(Mem.nextblock)=m1'.(Mem.nextblock))
                (CONT: Content_EI_Property j m1 m1' m2 (m2'.(Mem.mem_contents)))
-               (ACCESS: AccessMap_EI_Property m1 m1' m2 (m2'.(Mem.mem_access))),
+               (ACCESS: AccessMap_EI_Property j m1 m1' m2 (m2'.(Mem.mem_access))),
         mem_forward m2 m2' /\ 
-               Mem.extends m1' m2' /\ extends_perm_nonempty m1' m2' /\
-               Mem.inject j' m2' m3' /\  inject_perm_nonempty j' m2' m3' /\
+               Mem.extends m1' m2' /\ 
+               Mem.inject j' m2' m3' /\ 
                my_mem_unchanged_on (loc_out_of_bounds m1) m2 m2' /\
                my_mem_unchanged_on (loc_unmapped j) m2 m2' /\
                (mem_wd m2 -> mem_wd m2').
 Proof. intros.
-assert (VB: forall b, Mem.valid_block m1 b = Mem.valid_block m2 b).
-     intros. apply prop_ext. apply (Mem.valid_block_extends _ _ b Ext12). 
 assert (VB' : forall b : block, Mem.valid_block m1' b = Mem.valid_block m2' b).
   intros; unfold Mem.valid_block. rewrite NB. trivial.
 assert (Inj13:= extends_inject_compose _ _ _ _ Ext12 Inj23).
 assert (MMU_LU: my_mem_unchanged_on (loc_unmapped j) m2 m2' ).
-   split; intros. 
+   split. intros. 
        destruct (ACCESS b) as [Val _].
-        specialize (Val H k ofs).
-        apply (perm_split _ _ _ _ _ Val); clear Val; intros.
-            rewrite (perm_subst _ _ _ _ _ _ _ H1) in *. clear H1. 
-            rewrite <- VB in H.
-            destruct UnchOn1 as [UPerm _].
-                rewrite <- (UPerm _ _ _ HP H). eapply EP12. apply H0.
-         rewrite (perm_subst _ _ _ _ _ _ _ H1) in *. trivial.
-    assert (Val2:= Mem.perm_valid_block _ _ _ _ _ HMeperm).
-        destruct (ACCESS b) as [Val _].
-        specialize (Val Val2 Cur ofs).
-        destruct (CONT b) as [ContVal _].
-        destruct (ContVal Val2 ofs) as [ContValPerm ContValNoperm]; 
-                  clear ContVal.
-        apply (perm_split _ _ _ _ _ Val); clear Val; intros.
-            clear ContValNoperm.
-            specialize (ContValPerm H0). 
-            rewrite HP in ContValPerm.
-            rewrite ContValPerm; clear ContValPerm. trivial.
-        clear  ContValPerm.
-            rewrite (ContValNoperm H0). trivial.
-assert (EP12': extends_perm_nonempty m1' m2').
-      intros b2; intros.
-      assert (Val2': Mem.valid_block m2' b2). 
-             rewrite <-VB'. apply (Mem.perm_valid_block _ _ _ _ _ H).
-      apply (valid_split _ _ _ _  (ACCESS b2)); clear ACCESS; intros.
-           specialize (H1 k ofs).
-           apply (perm_split _ _ _ _ _ H1); clear H1; intros.
-              rewrite (perm_subst _ _ _ _ _ _ _ H2). trivial.
-           exfalso. apply H1. apply Fwd1. rewrite VB. apply H0.  apply H.
-      destruct (H1 k ofs) as [Val _]; clear H1.
-              rewrite (perm_subst _ _ _ _ _ _ _ (Val H)). trivial.
+        specialize (Val H k ofs). rewrite HP in Val.
+        rewrite (perm_subst _ _ _ _ _ _ _ Val). trivial.
+    intros. assert (Val2:= Mem.perm_valid_block _ _ _ _ _ HMeperm).
+        destruct (CONT b) as [ContVal _]. rewrite HP in ContVal.
+        rewrite (ContVal Val2 ofs). apply H. 
 assert (Fwd2: mem_forward m2 m2').
     split; intros.
      (*valid_block*) apply (Mem.valid_block_extends _ _ b Ext12) in H. 
@@ -116,22 +91,41 @@ assert (Fwd2: mem_forward m2 m2').
       (*max*)
       apply (valid_split _ _ _ _  (ACCESS b)); clear ACCESS; intros.
            specialize (H2 Max ofs).
-           apply (perm_split _ _ _ _ _ H2); clear H2; intros.
-              rewrite (perm_subst _ _ _ _ _ _ _ H3) in *. 
-              rewrite EP12. apply Fwd1. rewrite VB; trivial. trivial.
-                                      apply H2.
-           rewrite (perm_subst _ _ _ _ _ _ _ H3) in *. apply H0. 
+           remember (j b) as jb.
+           destruct jb; apply eq_sym in Heqjb.
+                destruct p0.
+                apply (perm_split _ _ _ _ _ _ _ H2); clear H2; intros.
+                    rewrite (perm_subst _ _ _ _ _ _ _ H3) in *. clear H3.
+                    unfold Mem.perm. rewrite po_oo in *.
+                       eapply po_trans. apply (extends_permorder _ _ Ext12).
+                       destruct (Fwd1 b). apply (Mem.perm_valid_block _ _ _ _ _ H2).
+                       apply (H4 ofs _ H0).
+                   rewrite (perm_subst _ _ _ _ _ _ _ H3) in *. apply H0.
+            rewrite (perm_subst _ _ _ _ _ _ _ H2) in *. apply H0.
       exfalso. apply (H1 H).
 assert (MMU_LOOB: my_mem_unchanged_on (loc_out_of_bounds m1) m2 m2'). 
    split; intros.
       apply (valid_split _ _ _ _  (ACCESS b)); clear ACCESS; intros.
-           destruct (H1 k ofs) as [_ Inval]; clear H1.
-           rewrite (perm_subst _ _ _ _ _ _ _ (Inval HP)). trivial.
+         specialize (H1 k ofs).
+         remember (j b) as jb.
+         destruct jb; apply eq_sym in Heqjb.
+              destruct p.
+              destruct H1 as [_ NoMax].
+              rewrite (perm_subst _ _ _ _ _ _ _ (NoMax HP)). trivial.
+         rewrite (perm_subst _ _ _ _ _ _ _ H1) in *. trivial.
       exfalso. apply (H0 H).
-  destruct (CONT b) as [Val _].
-      destruct (Val (Mem.perm_valid_block _ _ _ _ _ HMeperm) ofs)
-               as [_ NoPerm]; clear Val.
-      rewrite (NoPerm HP). assumption.
+  destruct (CONT b) as [ValC _].
+       destruct (ACCESS b) as [ValA _].
+       specialize (ValC (Mem.perm_valid_block _ _ _ _ _ HMeperm) ofs).
+       specialize (ValA (Mem.perm_valid_block _ _ _ _ _ HMeperm) Cur ofs).
+       unfold loc_out_of_bounds in HP.
+       remember (j b) as jb.
+       destruct jb; apply eq_sym in Heqjb.
+          destruct p.
+          eapply (perm_split _ _ _ _ _ _ _ ValC); clear ValC; intros.
+             exfalso. apply HP. apply H0.
+         rewrite H1. assumption.
+      rewrite ValC. assumption.
 split; trivial.
 assert (Ext12':  Mem.extends m1' m2').
     split. 
@@ -142,13 +136,23 @@ assert (Ext12':  Mem.extends m1' m2').
                                             Mem.perm m2' b ofs k p).
               intros. 
               apply (valid_split _ _ _ _  (ACCESS b)); clear ACCESS; intros.
-                  assert (Val1: Mem.valid_block m1 b). rewrite VB. trivial.
+                  assert (Val1: Mem.valid_block m1 b).
+                     apply (Mem.valid_block_extends _ _ _ Ext12). apply H0.
                   assert (Perm1: Mem.perm m1 b ofs Max Nonempty).
                         apply Fwd1. apply Val1.
                         eapply Mem.perm_max. eapply Mem.perm_implies.
                         apply H. constructor.
-                  destruct (H1 k ofs) as [Val _]; clear H1.
-                     rewrite (perm_subst _ _ _ _ _ _ _ (Val Perm1)). assumption.
+                  specialize (H1 k ofs).
+                  remember (j b) as jb.
+                  destruct jb; apply eq_sym in Heqjb.
+                     destruct p0.
+                     apply (perm_split _ _ _ _ _ _ _ H1); clear H1; intros.  
+                        rewrite (perm_subst _ _ _ _ _ _ _ H2). assumption.
+                      exfalso. apply (H1 Perm1). (*rewrite (perm_subst _ _ _ _ _ _ _ H2). assumption.*)
+            rewrite (perm_subst _ _ _ _ _ _ _ H1) in *. clear H1.
+                 destruct UnchOn1 as [UP _].
+                 eapply (extends_perm _ _ Ext12).
+                 rewrite (UP _ _ _ Heqjb Val1). apply H. 
              destruct (H1 k ofs) as [Val _]; clear H1.
                   assert (Perm1: Mem.perm m1' b ofs Max Nonempty). 
                           eapply Mem.perm_max. eapply Mem.perm_implies.
@@ -166,90 +170,30 @@ assert (Ext12':  Mem.extends m1' m2').
             destruct (CONT b2) as [ContVal ContInval]; clear CONT.
             apply (valid_split _ _ _ _  (ACCESS b2)); clear ACCESS; intros.
                 clear ContInval.
-                destruct (ContVal H ofs) as [ContVperm ContVNoPerm];
-                         clear ContVal.
-                specialize (H1 Cur ofs).
-                apply (perm_split _ _ _ _ _ H1); clear H1; intros.
-                     clear  ContVNoPerm.
-                     specialize (ContVperm H1).
-                     remember (j b2) as jb.
-                     destruct jb; apply eq_sym in Heqjb.
-                         destruct p. rewrite ContVperm. 
-                                     apply memval_inject_id_refl.
-                     rewrite ContVperm; clear ContVperm.
-                         destruct UnchOn1 as [U1Perm U1Val].
-                         assert (Val1:= Mem.perm_valid_block _ _ _ _ _ H1).
-                         assert (Perm1Cur:  Mem.perm m1 b2 ofs Cur Readable).
-                             rewrite U1Perm. apply H0. apply Heqjb. apply Val1.
-                         specialize (Mem.mi_memval _ _ _ (Mem.mext_inj _ _ 
-                                      Ext12) b2 ofs _ _ (eq_refl _) Perm1Cur).
-                         rewrite Zplus_0_r; intros.
-                         rewrite (U1Val _ _ Heqjb Perm1Cur _ (eq_refl _)).
-                         apply H3.
-                   clear  ContVperm ContVNoPerm H2.
-                        exfalso. apply H1; clear H1.
-                        apply Fwd1. rewrite VB. apply H. eapply Mem.perm_max. 
-                                    eapply Mem.perm_implies. apply H0.
-                                    constructor.
-             clear ContVal H1.
-                destruct (ContInval H ofs) as [ContVperm _]; clear ContInval.
-                rewrite ContVperm. apply memval_inject_id_refl.
-                       eapply Mem.perm_max. eapply Mem.perm_implies.
+                assert (Perm: Mem.perm m1 b2 ofs Max Nonempty).
+                    clear H1 ContVal. apply Fwd1.
+                     apply (Mem.valid_block_extends _ _ _ Ext12). apply H.
+                    eapply Mem.perm_max. eapply Mem.perm_implies.
                        apply H0. constructor.
+               specialize (ContVal H ofs). specialize (H1 Cur ofs).
+                  remember (j b2) as jb2.
+                  destruct jb2; apply eq_sym in Heqjb2.
+                          destruct p.
+                          destruct ContVal as [Cont _]. rewrite (Cont Perm). clear Cont.
+                          apply memval_inject_id_refl.
+                  rewrite ContVal. clear ContVal.
+                         destruct UnchOn1 as [UP UV].
+                         apply (Mem.valid_block_extends _ _ _ Ext12) in H.
+                         rewrite <- (UP _ _ _ Heqjb2 H) in H0.
+                         rewrite (UV _ _ Heqjb2 H0 _ (eq_refl _)).
+                         specialize (Mem.mi_memval _ _ _ (Mem.mext_inj _ _ 
+                                      Ext12) b2 ofs _ _ (eq_refl _) H0).
+                         rewrite Zplus_0_r; trivial.  
+                destruct (ContInval H ofs) as [Cont _]. 
+                  clear ContVal ContInval.
+                  rewrite (Cont H0); clear Cont. 
+                  apply memval_inject_id_refl.
 split; trivial.
-split; trivial.
-assert (IP23': inject_perm_nonempty j' m2' m3').
-    intros b; intros.
-    apply (valid_split _ _ _ _  (ACCESS b)); clear ACCESS; intros.
-        assert (Val1: Mem.valid_block m1 b). rewrite VB. trivial.
-        assert (J: j b = Some (b2, delta)).
-            remember (j b) as d. destruct d; apply eq_sym in Heqd. 
-              destruct p. rewrite (InjInc _ _ _ Heqd) in F.  apply F. 
-            destruct (injSep _ _ _ Heqd F). exfalso. apply (H1 Val1).
-        destruct (H0 Max ofs) as [Perm2'MaxP Perm2'MaxNop].
-        specialize (H0 k ofs).
-        apply (perm_split _ _ _ _ _ H0); clear H0; intros.
-            clear Perm2'MaxNop.
-            rewrite (perm_subst _ _ _ _ _ _ _ H1); clear H1. 
-            rewrite (perm_subst _ _ _ _ _ _ _ (Perm2'MaxP H0))
-               in NP; clear Perm2'MaxP.
-            apply IP13'. apply NP. apply F.
-        clear Perm2'MaxP.
-            rewrite (perm_subst _ _ _ _ _ _ _ H1); clear H1. 
-            rewrite (perm_subst _ _ _ _ _ _ _ (Perm2'MaxNop H0)) 
-               in NP; clear Perm2'MaxNop.
-            destruct UnchOn3 as [U3Perm _].
-            assert (loc_out_of_reach j m1 b2 (ofs + delta)).
-                unfold loc_out_of_reach; intros. intros N.
-                   destruct (eq_block b0 b); subst.
-                       rewrite H1 in J; inv J.
-                       assert (ofs + delta - delta = ofs). omega.
-                       rewrite H2 in N. apply (H0 N).
-                   assert (N2:Mem.perm m2 b0 (ofs+delta-delta0) Max Nonempty).
-                      rewrite EP12. apply N. apply N.
-                   destruct (Mem.mi_no_overlap _ _ _ Inj23 _ _ _ _ _ _ _ _ 
-                                               n H1 J N2 NP).
-                        apply H2; trivial.
-                        apply H2. omega.
-            assert (Val3: Mem.valid_block m3 b2). 
-                apply (Mem.valid_block_inject_2 _ _ _ _ _ _ J Inj23).
-            rewrite <- (U3Perm _ _ _ H1 Val3).
-            apply IP23. apply NP. apply J.
-   assert (NVal1: ~Mem.valid_block m1 b). rewrite VB. trivial.
-        assert (J: j b = None).
-            remember (j b) as d. destruct d; apply eq_sym in Heqd; trivial. 
-              destruct p. exfalso. apply H. 
-                       apply (Mem.valid_block_inject_1 _ _ _ _ _ _ Heqd Inj23).
-        destruct (H0 Max ofs) as [Perm2'MaxP Perm2'MaxNop].
-        specialize (H0 k ofs).
-        apply (perm_split _ _ _ _ _ H0); clear H0; intros.
-            clear Perm2'MaxNop.
-            rewrite (perm_subst _ _ _ _ _ _ _ H1); clear H1. 
-            rewrite (perm_subst _ _ _ _ _ _ _ (Perm2'MaxP H0)) in NP; 
-                    clear Perm2'MaxP.
-            apply IP13'. apply NP. apply F.
-        clear Perm2'MaxP.
-            unfold Mem.perm in NP. rewrite (Perm2'MaxNop H0) in NP. inv NP. 
 assert (Inj23': Mem.inject j' m2' m3').
     assert (MI: Mem.mem_inj j' m2' m3').
         assert (MiPerm: forall b1 b2 delta ofs k p,  j' b1 = Some (b2, delta) ->
@@ -259,14 +203,16 @@ assert (Inj23': Mem.inject j' m2' m3').
           assert (NP: Mem.perm m2' b1 ofs Max Nonempty).
             eapply Mem.perm_max. eapply Mem.perm_implies. apply H0. constructor.
           apply (valid_split _ _ _ _  (ACCESS b1)); clear ACCESS; intros.
-              assert (Val1: Mem.valid_block m1 b1). rewrite VB. trivial.
+              assert (Val1: Mem.valid_block m1 b1).
+                 apply (Mem.valid_block_extends _ _ _ Ext12). apply H1.
               assert (J: j b1 = Some (b2, delta)).
                   remember (j b1) as d. destruct d; apply eq_sym in Heqd. 
                     destruct p0. rewrite (InjInc _ _ _ Heqd) in H.  apply H. 
                   destruct (injSep _ _ _ Heqd H). exfalso. apply (H3 Val1).
+              rewrite J in H2.
               destruct (H2 Max ofs) as [Perm2'MaxP Perm2'MaxNop].
               specialize (H2 k ofs).
-              apply (perm_split _ _ _ _ _ H2); clear H2; intros.
+              apply (perm_split _ _ _ _ _ _ _ H2); clear H2; intros.
                   clear Perm2'MaxNop.
                   rewrite (perm_subst _ _ _ _ _ _ _ H3) in *; clear H3. 
                   eapply Inj13'. apply H. apply H0.
@@ -282,28 +228,31 @@ assert (Inj23': Mem.inject j' m2' m3').
                                assert (ofs + delta - delta = ofs). omega.
                                rewrite H4 in N. apply (H2 N).
                            assert (N2: Mem.perm m2 b0 (ofs + delta - delta0) 
-                                       Max Nonempty).
-                              rewrite EP12. apply N. apply N.
+                                       Max Nonempty). 
+                               specialize (Mem.mi_perm _ _ _ (Mem.mext_inj _ _  Ext12) b0 b0 Z0 
+                                                      (ofs + delta - delta0)). rewrite Zplus_0_r. intros. 
+                               apply (H4 _ _ (eq_refl _) N).
                            destruct (Mem.mi_no_overlap _ _ _ Inj23 _ _
                                                  _ _ _ _ _ _ n H3 J N2 NP).
                               apply H4; trivial.
                               apply H4. omega.
                   assert (Val3:=Mem.valid_block_inject_2 _ _ _ _ _ _ J Inj23).
               rewrite <- (U3Perm _ _ _ H3 Val3).
-              rewrite (IP23 b1). apply H0.  apply NP. apply J.
-          assert (NVal1: ~Mem.valid_block m1 b1). rewrite VB. trivial.
+                eapply Inj23. apply J. apply H0.
+          assert (NVal1: ~Mem.valid_block m1 b1). intros N. apply H1.
+                 apply (Mem.valid_block_extends _ _ _ Ext12). apply N.
           assert (J: j b1 = None).
               remember (j b1) as d. destruct d; apply eq_sym in Heqd; trivial.
                   destruct p0. exfalso. apply H1.
                      apply (Mem.valid_block_inject_1 _ _ _ _ _ _ Heqd Inj23).
           destruct (H2 Max ofs) as [Perm2'MaxP Perm2'MaxNop].
           specialize (H2 k ofs).
-          apply (perm_split _ _ _ _ _ H2); clear H2; intros.
+          apply (perm_split _ _ _ _ _ _ _ H2); clear H2; intros.
               clear Perm2'MaxNop.
               rewrite (perm_subst _ _ _ _ _ _ _ H3) in *; clear H3. 
               rewrite (perm_subst _ _ _ _ _ _ _ (Perm2'MaxP H2)) in NP; 
                       clear Perm2'MaxP.
-              rewrite (IP13' b1). apply H0. apply NP. apply H.
+              eapply Inj13'. apply H. apply H0.
           clear Perm2'MaxP.
               unfold Mem.perm in NP. 
               rewrite (Perm2'MaxNop H2) in NP. inv NP. 
@@ -330,17 +279,18 @@ assert (Inj23': Mem.inject j' m2' m3').
                    apply H0. constructor.
            apply (valid_split _ _ _ _  (ACCESS b1)); clear ACCESS; intros.
               clear ContInval.
-              destruct (ContVal H1 ofs) as [ContPerm ContNoPerm]; clear ContVal.
-              assert (Val1: Mem.valid_block m1 b1). rewrite VB. trivial.
+              specialize (ContVal H1 ofs).
+              apply (Mem.valid_block_extends _ _ _ Ext12) in H1.
               assert (J: j b1 = Some (b2, delta)).
                   remember (j b1) as d. destruct d; apply eq_sym in Heqd. 
                     destruct p. rewrite (InjInc _ _ _ Heqd) in H.  apply H. 
-                  destruct (injSep _ _ _ Heqd H). exfalso. apply (H3 Val1).
-              rewrite J in ContPerm.
+                  destruct (injSep _ _ _ Heqd H). exfalso. apply (H3 H1).
+              rewrite J in ContVal. destruct ContVal as [ContPerm ContNoperm].
+              rewrite J in H2.
               destruct (H2 Max ofs) as [Perm2'MaxP Perm2'MaxNop].
               specialize (H2 Cur ofs).
-              apply (perm_split _ _ _ _ _ H2); clear H2; intros.
-                  clear Perm2'MaxNop ContNoPerm.
+              apply (perm_split _ _ _ _ _ _ _ H2); clear H2; intros.
+                  clear Perm2'MaxNop ContNoperm.
                   rewrite (perm_subst _ _ _ _ _ _ _ H3) in *; clear H3.
                   rewrite (ContPerm H2). clear ContPerm. 
                   rewrite (perm_subst _ _ _ _ _ _ _ (Perm2'MaxP H2)) in *; 
@@ -350,7 +300,7 @@ assert (Inj23': Mem.inject j' m2' m3').
                   rewrite (perm_subst _ _ _ _ _ _ _ H3) in *; clear H3. 
                   rewrite (perm_subst _ _ _ _ _ _ _ (Perm2'MaxNop H2)) in *; 
                           clear Perm2'MaxNop.
-                  rewrite (ContNoPerm H2). clear ContNoPerm. 
+                  rewrite (ContNoperm H2). clear ContNoperm. 
                   destruct UnchOn3 as [U3Perm U3Val].
                   assert (loc_out_of_reach j m1 b2 (ofs + delta)).
                     unfold loc_out_of_reach; intros. intros N.
@@ -360,21 +310,25 @@ assert (Inj23': Mem.inject j' m2' m3').
                            rewrite H4 in N. apply (H2 N).
                        assert (N2: Mem.perm m2 b0 (ofs + delta - delta0) 
                                    Max Nonempty).
-                          rewrite EP12. apply N. apply N.
+                          (*rewrite EP12. apply N. apply N.*)
+                               specialize (Mem.mi_perm _ _ _ (Mem.mext_inj _ _  Ext12) b0 b0 Z0 
+                                                      (ofs + delta - delta0)). rewrite Zplus_0_r. intros. 
+                               apply (H4 _ _ (eq_refl _) N).
                        destruct (Mem.mi_no_overlap _ _ _ Inj23 _ _ _ 
                                                    _ _ _ _ _ n H3 J N2 NP).
                               apply H4; trivial.
                               apply H4. omega.
               assert (Val3:=Mem.valid_block_inject_2 _ _ _ _ _ _ J Inj23).
               assert (Perm3:  Mem.perm m3 b2 (ofs+delta) Cur Readable).
-                    rewrite (IP23 b1). apply H0. apply NP. apply J.
-              rewrite (U3Val _ _ H3 Perm3 _ (eq_refl _)).
+                  eapply Inj23. apply J. apply H0.                   
+            rewrite (U3Val _ _ H3 Perm3 _ (eq_refl _)).
               eapply memval_inject_incr.
                  apply (Mem.mi_memval _ _ _ (Mem.mi_inj _ _ _ Inj23) 
                                       _ _ _ _ J H0).
                    assumption. 
            clear ContVal. 
-              assert (NVal1: ~Mem.valid_block m1 b1). rewrite VB. trivial.
+              assert (NVal1: ~Mem.valid_block m1 b1). intros N. apply H1.
+                   apply (Mem.valid_block_extends _ _ _ Ext12). apply N.
               assert (J: j b1 = None).
                 remember (j b1) as d. 
                 destruct d; apply eq_sym in Heqd; trivial. 
@@ -384,12 +338,12 @@ assert (Inj23': Mem.inject j' m2' m3').
               destruct (ContInval H1 ofs) as [ContPerm ContNoPerm]; 
                        clear ContInval.
               specialize (H2 Cur ofs).
-              apply (perm_split _ _ _ _ _ H2); clear H2; intros.
+              apply (perm_split _ _ _ _ _ _ _ H2); clear H2; intros.
                   clear Perm2'MaxNop ContNoPerm.
                   rewrite (perm_subst _ _ _ _ _ _ _ H3) in *; clear H3. 
                   rewrite (perm_subst _ _ _ _ _ _ _ (Perm2'MaxP H2)) in NP; 
                           clear Perm2'MaxP.
-                  rewrite (ContPerm H2); clear ContPerm.
+                  rewrite (ContPerm H0); clear ContPerm.
                   eapply Inj13'. apply H. apply H0.
               clear Perm2'MaxP ContPerm.
                   unfold Mem.perm in NP. 
@@ -438,14 +392,16 @@ assert (Inj23': Mem.inject j' m2' m3').
               (*j b2 = None*)
                  destruct (injSep _ _ _ Heqjb2 H1). 
                  apply (valid_split _ _ _ _  (ACCESS b1)); intros.
-                     exfalso. rewrite <- VB in H8. apply (H4 H8).
+                     exfalso. apply H4. 
+                        apply (Mem.valid_block_extends _ _ _ Ext12). apply H8. 
                  specialize (H9 Max ofs1).
                  apply (valid_split _ _ _ _  (ACCESS b2)); intros.
-                     exfalso. rewrite <- VB in H10. apply (H6 H10).
+                     exfalso. apply H6. 
+                        apply (Mem.valid_block_extends _ _ _ Ext12). apply H10.
                  specialize (H11 Max ofs2).
-                 apply (perm_split _ _ _ _ _ H9); clear H9; intros.
+                 apply (perm_split _ _ _ _ _ _ _ H9); clear H9; intros.
                     rewrite (perm_subst _ _ _ _ _ _ _ H12) in *; clear H12.
-                    apply (perm_split _ _ _ _ _ H11); clear H11; intros.
+                    apply (perm_split _ _ _ _ _ _ _ H11); clear H11; intros.
                        rewrite (perm_subst _ _ _ _ _ _ _ H12) in *; clear H12.
                        eapply (Mem.mi_no_overlap _ _ _ Inj13' _ _ _
                                  _ _ _  _ _ H H0 H1 H2 H3).
@@ -458,9 +414,10 @@ assert (Inj23': Mem.inject j' m2' m3').
                remember (j b) as d. destruct d; apply eq_sym in Heqd. 
                  destruct p0. rewrite (InjInc _ _ _ Heqd) in H.  apply H.   
                  destruct (injSep _ _ _ Heqd H). exfalso. 
-                 rewrite VB in H3. apply (H3 H1).
+                 apply (Mem.valid_block_extends _ _ _ Ext12) in H1. apply (H3 H1).
              specialize (H2 k (Int.unsigned ofs)).
-             apply (perm_split _ _ _ _ _ H2); clear H2; intros.
+             rewrite J in H2.
+             apply (perm_split _ _ _ _ _ _ _ H2); clear H2; intros.
                    rewrite (perm_subst _ _ _ _ _ _ _ H3) in *; clear H3.
                    eapply Inj13'. apply H. apply H0.
              rewrite (perm_subst _ _ _ _ _ _ _ H3) in *; clear H3.
@@ -471,11 +428,10 @@ assert (Inj23': Mem.inject j' m2' m3').
                   destruct p0. exfalso. apply H1.
                   apply (Mem.valid_block_inject_1 _ _ _ _ _ _ Heqd Inj23).
              specialize (H2 k (Int.unsigned ofs)).
-             apply (perm_split _ _ _ _ _ H2); clear H2; intros.
+             apply (perm_split _ _ _ _ _ _ _ H2); clear H2; intros.
                  rewrite (perm_subst _ _ _ _ _ _ _ H3) in *; clear H3.
                      eapply Inj13'. apply H. apply H0.
              unfold Mem.perm in H0. rewrite H3 in H0. inv H0.
-split; trivial.
 split; trivial.
 split; trivial.
 split; trivial.
@@ -488,56 +444,54 @@ split; trivial.
       apply (valid_split _ _ _ _  (ACCESS b)); intros.
       (*case valid*)
           clear ContInval.
-          destruct (ContVal H0 ofs) as [ContPerm ContNoperm]; clear ContVal.
+          specialize (ContVal H0 ofs).
           specialize (H1 Cur ofs).
-          apply (perm_split _ _ _ _ _ H1); clear H1; intros.
-            rewrite (perm_subst _ _ _ _ _ _ _ H2) in *; clear H2.
-            clear ContNoperm.
-            specialize (ContPerm H1).
-            remember (j b) as jb.
-            destruct jb.
-               destruct p. rewrite ContPerm in Heqv; clear ContPerm.
+          remember (j b) as jb.
+          destruct jb; apply eq_sym in Heqjb.
+              destruct p. 
+              destruct ContVal as [ContPerm ContNoperm].
+              apply (perm_split _ _ _ _ _ _ _ H1); clear H1; intros.
+                rewrite (perm_subst _ _ _ _ _ _ _ H2) in *; clear H2.
+                clear ContNoperm.
+                rewrite (ContPerm H1) in Heqv; clear ContPerm.
                   unfold Mem.valid_block in VB'. 
                   rewrite <-  VB'. unfold mem_wd in WD1'.
                   assert (X: Mem.flat_inj (Mem.nextblock m1') b = Some (b, Z0)).
-                     apply flatinj_I. apply eq_sym in Heqjb. apply Fwd1.
+                     apply flatinj_I. apply Fwd1.
                      apply (Mem.valid_block_inject_1 _ _ _ _ _ _ Heqjb Inj13).
                   destruct WD1'. specialize (mi_memval b ofs _ _ X R). 
                   rewrite Zplus_0_r in mi_memval. 
                   rewrite <- Heqv in mi_memval.
                   clear X Heqv. inversion mi_memval. clear H8. 
                   subst. apply flatinj_E in H4. apply H4.
-            rewrite ContPerm in Heqv; clear ContPerm.
-                  assert (X: Mem.flat_inj (Mem.nextblock m2) b = Some (b, Z0)).
+            clear ContPerm.
+              rewrite (perm_subst _ _ _ _ _ _ _ H2) in *; clear H2.
+              rewrite (ContNoperm H1) in Heqv; clear ContNoperm.
+              assert (X: Mem.flat_inj (Mem.nextblock m2) b = Some (b, Z0)).
+                         apply flatinj_I. apply H0.
+              destruct WD2. specialize (mi_memval b ofs _ _ X R). 
+              rewrite Zplus_0_r in mi_memval. rewrite <- Heqv in mi_memval.
+              clear X Heqv. inversion mi_memval. clear H8. subst. 
+              apply flatinj_E in H4.
+              apply Fwd2. apply H4.
+         (*j b = None*)
+           rewrite ContVal in Heqv. clear ContVal.
+           rewrite (perm_subst _ _ _ _ _ _ _ H1) in R; clear H1.
+           assert (X: Mem.flat_inj (Mem.nextblock m2) b = Some (b, Z0)).
                                    apply flatinj_I. apply H0.
-                  assert (R2: Mem.perm m2 b ofs Cur Readable).
-                     rewrite EP12; try apply H1.
-                     destruct UnchOn1 as [U1Perm _]. 
-                     rewrite U1Perm. apply R. 
-                     unfold loc_unmapped. rewrite Heqjb. trivial.
-                     apply (Mem.perm_valid_block _ _ _ _ _ H1).
-                  destruct WD2. specialize (mi_memval b ofs _ _ X R2). 
+             destruct WD2. specialize (mi_memval b ofs _ _ X R). 
                   rewrite Zplus_0_r in mi_memval. rewrite <- Heqv in mi_memval.
-                  clear X Heqv. inversion mi_memval. clear H8. 
-                  subst. apply flatinj_E in H4.
-                  apply Fwd2.  apply H4.
-          clear ContPerm.
-            rewrite (perm_subst _ _ _ _ _ _ _ H2) in *; clear H2.
-            rewrite (ContNoperm H1) in Heqv; clear ContNoperm.
-            assert (X: Mem.flat_inj (Mem.nextblock m2) b = Some (b, Z0)).
-                       apply flatinj_I. apply H0.
-            destruct WD2. specialize (mi_memval b ofs _ _ X R). 
-            rewrite Zplus_0_r in mi_memval. rewrite <- Heqv in mi_memval.
-            clear X Heqv. inversion mi_memval. clear H8. subst. 
-            apply flatinj_E in H4.
-            apply Fwd2. apply H4.
-      clear ContVal.
+                  clear X Heqv. inversion mi_memval. clear H7. 
+                  subst. apply flatinj_E in H3.
+                  apply Fwd2.  apply H3.
+      (*case invalid*)
+        clear ContVal.
         destruct (ContInval H0 ofs) as [ContPerm ContNoperm]; clear ContInval.
         specialize (H1 Cur ofs).
-        apply (perm_split _ _ _ _ _ H1); clear H1; intros.
+        apply (perm_split _ _ _ _ _ _ _ H1); clear H1; intros.
            rewrite (perm_subst _ _ _ _ _ _ _ H2) in *; clear H2.
            clear ContNoperm.
-           rewrite (ContPerm H1) in Heqv; clear ContPerm.
+           rewrite (ContPerm R) in Heqv; clear ContPerm.
            assert (X: Mem.flat_inj (Mem.nextblock m1') b = Some (b, Z0)).
                   apply flatinj_I. apply (Mem.perm_valid_block _ _ _ _ _ H1).
            destruct WD1'. specialize (mi_memval b ofs _ _ X R). 
@@ -549,10 +503,10 @@ split; trivial.
     rewrite Int.add_zero. trivial.
 Qed.
 
-Parameter mkAccessMap_EI_exists:  forall  (m1 m1' m2:Mem.mem), 
+Parameter mkAccessMap_EI_exists:  forall (j:meminj) (m1 m1' m2:Mem.mem), 
           ZMap.t (Z -> perm_kind -> option permission).
-Axiom mkAccessMap_EI_ok: forall  (m1 m1' m2:Mem.mem), 
-      AccessMap_EI_Property m1 m1' m2 (mkAccessMap_EI_exists m1 m1' m2).
+Axiom mkAccessMap_EI_ok: forall j (m1 m1' m2:Mem.mem), 
+      AccessMap_EI_Property j m1 m1' m2 (mkAccessMap_EI_exists j m1 m1' m2).
 
 Parameter mkContentsMap_EI_exists: 
            forall (j :meminj) (m1 m1' m2:Mem.mem), ZMap.t (ZMap.t memval).
@@ -560,36 +514,42 @@ Axiom mkContentsMap_EI_ok: forall j m1 m1' m2,
       Content_EI_Property j m1 m1' m2 (mkContentsMap_EI_exists j m1 m1' m2).
 
 Definition mkEI (j j': meminj) (m1 m2 m1':mem)
-                (Ext12: Mem.extends m1 m2) (EP12: extends_perm_nonempty m1 m2)
+                (Ext12: Mem.extends m1 m2) 
                 (Fwd1: mem_forward m1 m1') m3 
-                (Inj23: Mem.inject j m2 m3) (IP23: inject_perm_nonempty j m2 m3)
+                (Inj23: Mem.inject j m2 m3)
                 m3' (Fwd3: mem_forward m3 m3') 
                 (Inj13': Mem.inject j' m1' m3')
-                (IP13': inject_perm_nonempty j' m1' m3')
                 (UnchOn3: my_mem_unchanged_on (loc_out_of_reach j m1) m3 m3') 
                 (InjInc: inject_incr j j') (injSep: inject_separated j j' m1 m3)
                 (UnchOn1: my_mem_unchanged_on (loc_unmapped j) m1 m1')
                 (WD1': mem_wd m1') (WD2: mem_wd m2) (WD3': mem_wd m3')
              : Mem.mem'.
 eapply Mem.mkmem with (nextblock:=m1'.(Mem.nextblock))
-                      (mem_access:=mkAccessMap_EI_exists m1 m1' m2).
+                      (mem_access:=mkAccessMap_EI_exists j m1 m1' m2).
   apply (mkContentsMap_EI_exists j m1 m1' m2).
   apply m1'.
   (*access_max*)
-     intros. specialize (mkAccessMap_EI_ok m1 m1' m2 b). intros.
+     intros. specialize (mkAccessMap_EI_ok j m1 m1' m2 b). intros.
      apply (valid_split _ _ _ _  H); clear H; intros.
      (*valid_block m2 b*)
-         destruct (H0 Max ofs) as [MaxPerm MaxNoPerm].
-         apply (perm_split _ _ _ _ _ (H0 Cur ofs)); clear H0; intros.
-              clear MaxNoPerm.
+         assert (MAX:= H0 Max ofs). 
+         specialize (H0 Cur ofs).
+         remember (j b) as jb.
+         destruct jb; apply eq_sym in Heqjb.
+            destruct p.
+            destruct MAX as [MaxPerm MaxNoperm].
+            apply (perm_split _ _ _ _ _ _ _ H0); clear H0; intros.
+              clear MaxNoperm.
                  rewrite H1 in *; clear H1.
                  rewrite (MaxPerm H0). apply m1'.
-          clear MaxPerm. 
+            clear MaxPerm. 
                  rewrite H1 in *; clear H1.
-                 rewrite (MaxNoPerm H0). apply m2.
+                 rewrite (MaxNoperm H0). apply m2.
+          rewrite H0 in *; clear H0.
+                 rewrite MAX; clear MAX. apply m2.
      (*~ valid_block m2 b*)
          destruct (H0 Max ofs) as [MaxPerm MaxNoPerm].
-         apply (perm_split _ _ _ _ _ (H0 Cur ofs)); clear H0; intros.
+         apply (perm_split _ _ _ _ _ _ _ (H0 Cur ofs)); clear H0; intros.
               clear MaxNoPerm.
                  rewrite H1 in *; clear H1.
                  rewrite (MaxPerm H0). apply m1'.
@@ -600,40 +560,39 @@ eapply Mem.mkmem with (nextblock:=m1'.(Mem.nextblock))
     intros. 
     assert (NV1' : ~ Mem.valid_block m1' b). apply H.
     assert (NV1 : ~ Mem.valid_block m1 b). intros N. destruct (Fwd1 _ N). apply (NV1' H0).
-    destruct (mkAccessMap_EI_ok m1 m1' m2 b) as [_ Inval].
+    destruct (mkAccessMap_EI_ok j m1 m1' m2 b) as [_ Inval].
      assert (NVB2: ~ Mem.valid_block m2 b). 
         intros N. apply NV1. 
         apply (Mem.valid_block_extends _ _ b Ext12). apply N.
      specialize (Inval NVB2 k ofs).
-     apply (perm_split _ _ _ _ _ Inval); clear Inval; intros.
+     apply (perm_split _ _ _ _ _ _ _ Inval); clear Inval; intros.
           rewrite H1. apply m1'.  apply H.
           rewrite H1. trivial.
 Defined.
 
 Lemma my_interpolate_EI: forall (j j': meminj) (m1 m2 m1':mem)
-                (Ext12: Mem.extends m1 m2) (EP12: extends_perm_nonempty m1 m2)
+                (Ext12: Mem.extends m1 m2) 
                 (Fwd1: mem_forward m1 m1') m3 
-                (Inj23: Mem.inject j m2 m3) (IP23: inject_perm_nonempty j m2 m3)
+                (Inj23: Mem.inject j m2 m3)
                 m3' (Fwd3: mem_forward m3 m3') 
                 (Inj13': Mem.inject j' m1' m3') 
-                (IP13': inject_perm_nonempty j' m1' m3')
                 (UnchOn3: my_mem_unchanged_on (loc_out_of_reach j m1) m3 m3') 
                 (InjInc: inject_incr j j') (injSep: inject_separated j j' m1 m3)
                 (UnchOn1: my_mem_unchanged_on (loc_unmapped j) m1 m1')
                 (WD1': mem_wd m1') (WD2: mem_wd m2) (WD3': mem_wd m3'),
     exists m2', mem_forward m2 m2' /\
-                Mem.extends m1' m2' /\  extends_perm_nonempty m1' m2' /\
-                Mem.inject j' m2' m3' /\  inject_perm_nonempty j' m2' m3' /\
+                Mem.extends m1' m2' /\ 
+                Mem.inject j' m2' m3' /\ 
                 my_mem_unchanged_on (loc_out_of_bounds m1) m2 m2' /\
                 my_mem_unchanged_on (loc_unmapped j) m2 m2' /\
                 (mem_wd m2 -> mem_wd m2').
 Proof. intros. 
-  exists (mkEI j j' m1 m2 m1' Ext12 EP12 Fwd1 _ Inj23 IP23 _ Fwd3 Inj13' IP13'
+  exists (mkEI j j' m1 m2 m1' Ext12 Fwd1 _ Inj23 _ Fwd3 Inj13' 
               UnchOn3 InjInc injSep UnchOn1 WD1' WD2 WD3'). 
-  apply (EI_ok m1 m2 m1' Ext12 EP12 Fwd1 _ _ Inj23 IP23 _ Fwd3 _ Inj13' IP13'
+  apply (EI_ok m1 m2 m1' Ext12 Fwd1 _ _ Inj23 _ Fwd3 _ Inj13'
             UnchOn3 InjInc injSep UnchOn1 WD1' WD2 WD3' 
-            (mkEI j j' m1 m2 m1' Ext12 EP12 Fwd1 m3 Inj23 IP23 m3' Fwd3 
-                  Inj13' IP13' UnchOn3 InjInc injSep UnchOn1 WD1' WD2 WD3')
+            (mkEI j j' m1 m2 m1' Ext12 Fwd1 m3 Inj23 m3' Fwd3 
+                  Inj13' UnchOn3 InjInc injSep UnchOn1 WD1' WD2 WD3')
             (eq_refl _)).
    apply mkContentsMap_EI_ok.  apply mkAccessMap_EI_ok.
 Qed.
@@ -654,12 +613,9 @@ Lemma interpolate_EI: forall (m1 m2 m1':mem)
                    mem_unchanged_on (loc_unmapped j) m2 m2' /\
                    (mem_wd m2 -> mem_wd m2').
 Proof. intros. rewrite <- unchAx in UnchOn3.  rewrite <- unchAx in UnchOn1. 
-  assert (EP12 := ext_implies_extends_perm_nonenempty _ _ Ext12).
-  assert (IP23 := inj_implies_inject_perm_nonenempty _ _ _ Inj23).
-  assert (IP13' := inj_implies_inject_perm_nonenempty _ _ _ Inj13').
-  destruct (my_interpolate_EI _ _ _ _ _ Ext12 EP12 Fwd1 _ Inj23 IP23 _ 
-              Fwd3 Inj13' IP13' UnchOn3 InjInc injSep UnchOn1 WD1' WD2 WD3')
-    as [m2' [Fwd2 [Ext12' [_ [Inj23' [_ [UnchLoob22 [UnchLU22 WD2']]]]]]]].
+  destruct (my_interpolate_EI _ _ _ _ _ Ext12 Fwd1 _ Inj23 _ 
+              Fwd3 Inj13' UnchOn3 InjInc injSep UnchOn1 WD1' WD2 WD3')
+    as [m2' [Fwd2 [Ext12' [Inj23' [UnchLoob22 [UnchLU22 WD2']]]]]].
   rewrite unchAx in *. 
   exists m2'. repeat (split; trivial).
 Qed.
