sepcomp/mem_interpolation_proofs.v
@@ -1,9 +1,9 @@
 Load loadpath.
 Require Import sepcomp.mem_interpolants.
-Require Import sepcomp.mem_interpolation_EE.
-Require Import sepcomp.mem_interpolation_EI.
-Require Import sepcomp.mem_interpolation_IE.
-Require Import sepcomp.mem_interpolation_II.
+Require Import sepcomp.i_EE.
+Require Import sepcomp.i_EI.
+Require Import sepcomp.i_IE.
+Require Import sepcomp.i_II.
 
 Module MemoryInterpolations <: MemoryInterpolationAxioms.
 Definition  interpolate_II := interpolate_II.
